Invariants proof
Updated invariants proof

Monad_Play Around/DNFP/Dutch_National_Flag_Monad.thy
@@ -18,13 +18,6 @@ fun dnfp_mon:: "nat \<Rightarrow> (env, unit) state" where
 
 section\<open>Lemmas\<close>
 subsection\<open>Hoare proofs\<close>
-
-definition loop_update_action_inv :: "env \<Rightarrow> bool" where
-"loop_update_action_inv s \<equiv> (loop_update_action_inv3 s \<and> loop_update_action_inv2 s \<and> loop_update_action_inv1 s)"
-
-lemma loop_update_action_invariants: "spec loop_update_action_inv loop_update_action (GG invariants_Env)"
-  by (metis (mono_tags, lifting) GG_def loop_update_action_inv_def loop_update_action_invariantBlue loop_update_action_invariantRed loop_update_action_invariantWhite invariants_Env_def spec_def split_def)
-
 subsection\<open>DNFP_Mon Auxillary lemmas\<close>
 lemma dnfp_aux1: "spec (\<lambda>y. length (xs e) = length (xs y)) (dnfp_mon v) (\<lambda>x y. length (xs e) = length (xs y))"
   apply(induction v rule: dnfp_mon.induct)
@@ -222,70 +215,100 @@ lemma dnfp_aux6: "spec (\<lambda>y. mset (xs e) = mset (xs y)) (dnfp_mon v) (\<l
   apply(intro seq_rule[of _ _ "(\<lambda>x y. mset (xs e) = mset (xs y))"])
   apply(intro cond_rule)
   apply(simp add: inc_lowbound_def)
-   apply(intro get_rule; intro allI; simp)
-  apply(intro seq_rule[of _ _ "(\<lambda>x y. mset (xs e) = mset (xs y))"])
-       apply(simp add: spec_def put_def xs_Env_def swap_def put_state_def get_state_def)
-  apply (simp add: Multiset.mset_swap)
-   apply(intro allI; simp)
-   apply(intro get_rule; intro allI)
-  apply(intro seq_rule[of _ _ "(\<lambda>x y. mset (xs e) = mset (xs y))"])
-    apply(simp add: spec_def put_def i_Env_def put_state_def get_state_def)
-   apply(intro allI; simp)
-         apply(intro get_rule; intro allI)
-    apply(simp add: spec_def put_def low_Env_def put_state_def get_state_def)
-  apply(simp add: dec_highbound_def)
-   apply(intro get_rule; intro allI; simp)
-  apply(intro seq_rule[of _ _ "(\<lambda>x y. mset (xs e) = mset (xs y))"])
-      apply(simp add: spec_def put_def high_Env_def put_state_def get_state_def)
-   apply(intro allI; simp)
   apply(intro get_rule; intro allI; simp)
-     apply(simp add: spec_def put_def xs_Env_def swap_def put_state_def get_state_def)
+  apply(intro seq_rule[of _ _ "(\<lambda>x y. mset (xs e) = mset (xs y))"])
+  apply(simp add: spec_def put_def xs_Env_def swap_def put_state_def get_state_def)
+  apply (simp add: Multiset.mset_swap)
+  apply(intro allI; simp)
+  apply(intro get_rule; intro allI)
+  apply(intro seq_rule[of _ _ "(\<lambda>x y. mset (xs e) = mset (xs y))"])
+  apply(simp add: spec_def put_def i_Env_def put_state_def get_state_def)
+  apply(intro allI; simp)
+  apply(intro get_rule; intro allI)
+  apply(simp add: spec_def put_def low_Env_def put_state_def get_state_def)
+  apply(simp add: dec_highbound_def)
+  apply(intro get_rule; intro allI; simp)
+  apply(intro seq_rule[of _ _ "(\<lambda>x y. mset (xs e) = mset (xs y))"])
+  apply(simp add: spec_def put_def high_Env_def put_state_def get_state_def)
+  apply(intro allI; simp)
+  apply(intro get_rule; intro allI; simp)
+  apply(simp add: spec_def put_def xs_Env_def swap_def put_state_def get_state_def)
   apply (simp add: Multiset.mset_swap)
   apply(simp add: inc_index_def)
   apply(intro get_rule; intro allI; simp)
-    apply(simp add: spec_def put_def i_Env_def put_state_def get_state_def)
-   apply blast
+  apply(simp add: spec_def put_def i_Env_def put_state_def get_state_def)
+  apply blast
   apply(simp add: spec_def)
   by (simp add: skip_def)
 
-lemma dnfp_aux7: "spec (\<lambda>y. i y \<le> high y) (dnfp_mon n) (\<lambda>x y. high y = i y)"
+lemma dnfp_aux7: "spec (\<lambda>y. i y \<le> high y \<and> high y - i y \<le> n) (dnfp_mon n) (\<lambda>x y. high y = i y)"
   apply(induction n rule: dnfp_mon.induct)
-    apply(simp add: spec_def)
-   apply (simp add: skip_def)
-  defer
-  apply(simp only: caseN)
+    apply(simp add: spec_def)    
+   apply (simp add: skip_def)    
+  apply(simp only: caseN)  
   apply(intro get_rule; intro allI; clarify)
   apply(intro cond_rule)
   apply(simp add: loop_update_action_def)
-  apply(intro get_rule; intro allI; clarify)
-  apply(intro seq_rule[of _ _ "(\<lambda>x y. i y \<le> high y)"])
-  apply(intro cond_rule)
-  apply(simp add: inc_lowbound_def)
-   apply(intro get_rule; intro allI; simp)
-  apply(intro seq_rule[of _ _ "(\<lambda>x y. i y < high y)"])
-    apply(simp add: spec_def put_def xs_Env_def swap_def put_state_def get_state_def)
-       apply(intro allI; simp)
-   apply(intro get_rule; intro allI)
-  apply(intro seq_rule[of _ _ "(\<lambda>x y. i y \<le> high y)"])
+  apply(intro get_rule; intro allI; clarify)            
+  apply(intro seq_rule[of _ _ "(\<lambda>x y. i y \<le> high y \<and> high y - i y \<le> n)"])
+     apply(intro conj_rule_right)              
+
+    apply(intro cond_rule)
+  apply(simp add: inc_lowbound_def)        
+   apply(intro get_rule; intro allI; simp)             
+  apply(intro seq_rule[of _ _ "(\<lambda>x y. i y < high y)"])          
+       apply(simp add: spec_def put_def xs_Env_def swap_def put_state_def get_state_def)    
+       apply(intro allI; simp)                                    
+   apply(intro get_rule; intro allI)                             
+  apply(intro seq_rule[of _ _ "(\<lambda>x y. i y \<le> high y)"])     
+       apply(simp add: spec_def put_def i_Env_def put_state_def get_state_def)
+       apply(intro allI; simp)                    
+     apply(intro get_rule; intro allI)                     
+       apply(simp add: spec_def put_def low_Env_def put_state_def get_state_def)    
+                                 
+     apply(simp add: dec_highbound_def)                 
+  apply(intro get_rule; intro allI; simp)              
+ apply(intro seq_rule[of _ _ "(\<lambda>x y. i y \<le> high y)"])        
+     apply(simp add: spec_def put_def high_Env_def put_state_def get_state_def)
+       apply linarith 
+         apply(intro allI; simp)            
+      apply(intro get_rule; intro allI; simp)                       
+     apply(simp add: spec_def put_def xs_Env_def put_state_def get_state_def)
+                                         
+     apply(simp add: inc_index_def)                
+      apply(intro get_rule; intro allI; simp)                       
     apply(simp add: spec_def put_def i_Env_def put_state_def get_state_def)
+
+    apply(intro cond_rule)
+      apply(simp add: inc_lowbound_def)                  
+      apply(intro get_rule; intro allI; simp)       
+(*I need some help here*)                                      
+ apply(intro seq_rule[of _ _ "(\<lambda>x y. high y - i y \<le> n \<and> high e = high y \<and> i e = i y)"])          
+      apply(simp add: spec_def put_def xs_Env_def swap_def put_state_def get_state_def)    
+  defer                               
        apply(intro allI; simp)
-     apply(intro get_rule; intro allI)
-    apply(simp add: spec_def put_def low_Env_def put_state_def get_state_def)
+  apply(intro get_rule; intro allI)                             
+ apply(intro seq_rule[of _ _ "(\<lambda>x y. high y - i y \<le> n)"])   
+      apply(simp add: spec_def put_def i_Env_def put_state_def get_state_def)
+  apply linarith                                    
+        apply(intro allI; simp)   
+    apply(intro get_rule; intro allI)
+      apply(simp add: spec_def put_def low_Env_def put_state_def get_state_def)    
+                                  
       apply(simp add: dec_highbound_def)
-   apply(intro get_rule; intro allI; simp)
-  apply(intro seq_rule[of _ _ "(\<lambda>x y. i y \<le> high y)"])
-      apply(simp add: spec_def put_def high_Env_def put_state_def get_state_def)
-  apply linarith
-   apply(intro allI; simp)
-  apply(intro get_rule; intro allI; simp)
-      apply(simp add: spec_def put_def xs_Env_def swap_def put_state_def get_state_def)
-  apply(simp add: inc_index_def)
-  apply(intro get_rule; intro allI; simp)
-    apply(simp add: spec_def put_def i_Env_def put_state_def get_state_def)
-      apply(intro allI; simp)
-  apply blast
+      apply(intro get_rule; intro allI; simp)          
+(*I need some help here*)
+  apply(intro seq_rule[of _ _ "(\<lambda>x y. high y - i y \<le> n)"])
+       apply(simp add: spec_def put_def high_Env_def put_state_def get_state_def)  
+
+       defer                        
+  defer
+      apply(simp add: inc_index_def)     
+  apply(intro get_rule; intro allI; simp) 
+       apply(simp add: spec_def put_def i_Env_def put_state_def get_state_def run_state_def)     
+  defer                                   
+      apply(intro allI; simp)    
    apply(simp add: spec_def put_def i_Env_def put_state_def get_state_def run_state_def)
-  apply (simp add: skip_def)
   sorry
 
 
@@ -424,7 +447,7 @@ lemma dnfp_prepost: "spec (dnfp_pre n e) (dnfp_mon n) (GG (dnfp_post e))"
   apply(intro seq_rule[of _ _ "(\<lambda>x y. high y - i y \<le> high e - i e)"])
        apply(intro cond_rule)
  apply(simp add: inc_lowbound_def)
-   apply(intro get_rule; intro allI; simp)
+   apply(intro get_rule; intro allI; simp)             
   apply(intro seq_rule[of _ _ "(\<lambda>x y. high y - i y \<le> high e - i e)"])
     apply(simp add: spec_def put_def xs_Env_def swap_def put_state_def get_state_def)
    apply(intro allI; simp)
@@ -434,7 +457,7 @@ lemma dnfp_prepost: "spec (dnfp_pre n e) (dnfp_mon n) (GG (dnfp_post e))"
   apply (simp add: le_diff_conv)
    apply(intro allI; simp)
    apply(intro get_rule; intro allI)
-    apply(simp add: spec_def put_def low_Env_def put_state_def get_state_def)
+  apply(simp add: spec_def put_def low_Env_def put_state_def get_state_def)
   apply(simp add: dec_highbound_def)
    apply(intro get_rule; intro allI; simp)
   apply(intro seq_rule[of _ _ "(\<lambda>x y. high y - i y \<le> high e - i e)"])
@@ -482,258 +505,104 @@ lemma dnfp_prepost: "spec (dnfp_pre n e) (dnfp_mon n) (GG (dnfp_post e))"
    apply(simp add: spec_def put_def i_Env_def put_state_def get_state_def)
     apply(intro allI; simp)
   using dnfp_aux6 apply blast
-   apply(simp add: spec_def skip_def)
-
- apply(intro get_rule; intro allI; clarify)
- apply(intro cond_rule)
-  apply(simp add: loop_update_action_def)
-  apply(intro get_rule; intro allI; clarify)
-  apply(intro seq_rule[of _ _ "(\<lambda>x y. high y \<ge> i y)"])
-       apply(intro cond_rule)
- apply(simp add: inc_lowbound_def)
-   apply(intro get_rule; intro allI; simp)
-  apply(intro seq_rule[of _ _ "(\<lambda>x y. high y > i y)"])
-  apply(simp add: spec_def put_def xs_Env_def swap_def put_state_def get_state_def)
-       apply(intro allI; simp)
-   apply(intro get_rule; intro allI)
-  apply(intro seq_rule[of _ _ "(\<lambda>x y. high y \<ge> i y)"])
-        apply(simp add: spec_def put_def i_Env_def put_state_def get_state_def)
-   apply(intro allI; simp)
-         apply(intro get_rule; intro allI)
-    apply(simp add: spec_def put_def low_Env_def put_state_def get_state_def)
-      apply(simp add: dec_highbound_def)
-   apply(intro get_rule; intro allI; simp)
-  apply(intro seq_rule[of _ _ "(\<lambda>x y. high y \<ge> i y)"])
-  apply(simp add: spec_def put_def high_Env_def put_state_def get_state_def)
-  apply linarith
-   apply(intro allI; simp)
-  apply(intro get_rule; intro allI; simp)
-  apply(simp add: spec_def put_def xs_Env_def swap_def put_state_def get_state_def)
-      apply(simp add: inc_index_def)
-  apply(intro get_rule; intro allI; simp)
-      apply(simp add: spec_def put_def i_Env_def put_state_def get_state_def)
-   apply(intro allI; simp)
-  using dnfp_aux7 apply blast 
   by(simp add: spec_def skip_def)
 
-subsection\<open>Invariants proof\<close>
+(*
+  add precondition:
+  Everything outside n is sorted
+  high to n
+  And finally everything should be sorted
+  Post condition high = i 
+*)
 
-subsubsection\<open>Lemmas\<close>
-lemma dnfp_invariantRed_aux: "spec (\<lambda>e. \<forall>x<low e. xs e ! x = 0) (dnfp_mon v) (\<lambda>x e. \<forall>x<low e. xs e ! x = 0)"
- apply(induction v rule: dnfp_mon.induct)
+definition pre_dnfp_mon where
+"pre_dnfp_mon n e \<equiv> high e - i e = n
+                    \<and> dnfp_precondition e
+                    \<and> high e - i e = n
+                    \<and> invariants_Env e "
+
+subsection\<open>Invariants proof\<close>
+lemma dnfp_invariantRed: "spec (dnfp_inv1) (dnfp_mon n) (GG dnfp_inv1)"
+  unfolding dnfp_inv1_def dnfp_pre_aux_def GG_def 
+  apply(induction n rule: dnfp_mon.induct)
     apply(simp add: spec_def)
-    apply (simp add: skip_def)
+    apply(simp add: skip_def)
   apply(simp only: caseN)
-  apply(intro get_rule; intro allI; clarify)
-  apply(intro cond_rule)
+   apply(intro get_rule; intro allI; clarify)
+  apply(intro cond_rule; simp)
+   apply(simp add: loop_update_action_def)
+   apply(intro get_rule; intro allI; clarify)
+  apply(intro seq_rule[of _ _ "(\<lambda>x e. dnfp_precondition e \<and> low_invariant_is_0_Env e)"])
+    apply(intro cond_rule)
+  apply (smt GG_def One_nat_def case_prodD case_prodI2 inc_lowbound_inv1_aux_def inc_lowbound_inv1_def inc_lowbound_invariantRed lessI loop_update_action_pre_def prod.simps(1) spec_def)
+  apply (smt GG_def case_prodD case_prodI2 dec_highbound_inv1_aux_def dec_highbound_inv1_def dec_highbound_invariantRed loop_update_action_pre_def prod.simps(1) spec_def)
+    apply (smt GG_def case_prodD case_prodI2 inc_index_inv1_aux_def inc_index_inv1_def inc_index_invariantRed less_one loop_update_action_pre_def prod.simps(1) spec_def) 
+   apply blast
+    apply(simp add: spec_def)
+   by(simp add: skip_def)
+
+lemma dnfp_invariantWhite: "spec dnfp_inv2 (dnfp_mon n) (GG dnfp_inv2)"
+  unfolding dnfp_inv2_def  GG_def dnfp_pre_aux_def
+  apply(induction n rule: dnfp_mon.induct)
+    apply(simp add: spec_def)
+    apply(simp add: skip_def)
+  apply(simp only: caseN)
+   apply(intro get_rule; intro allI; clarify)
+  apply(intro cond_rule; simp)
   apply(simp add: loop_update_action_def)
-  apply(intro get_rule; intro allI; clarify)
-  apply(intro seq_rule[of _ _ "(\<lambda>x e. (\<forall>x<low e. xs e ! x = 0))"])
-  apply(intro cond_rule)
-  apply(simp add: inc_lowbound_def)
-      apply (intro get_rule; intro allI; simp)
-  apply(intro seq_rule[of _ _ "(\<lambda>x e. xs e ! low e = 0 \<and> (\<forall>x<low e. xs e ! x = 0))"])
-       apply (simp add: spec_def put_def put_state_def swap_def get_state_def xs_Env_def)
-    (*Look here*)
-  apply(intro allI)
-  defer
-       apply(intro allI; simp)
-  apply(intro get_rule; intro allI)
-  apply(intro seq_rule[of _ _ "(\<lambda>x e. xs e ! low e = 0 \<and> (\<forall>x<low e. xs e ! x = 0))"])
-        apply (simp add: spec_def put_def put_state_def get_state_def i_Env_def)
-  apply(intro allI; simp)
-  apply(intro get_rule; intro allI)
-       apply (simp add: spec_def put_def put_state_def get_state_def low_Env_def)
-  apply (simp add: less_Suc_eq)
-     apply(simp add: dec_highbound_def)
-     apply (intro get_rule; intro allI; simp)
-      apply(intro seq_rule[of _ _ "(\<lambda>x e. low e \<le> i e \<and> i e \<le> high e \<and> (\<forall>x<low e. xs e ! x = 0))"]) 
-       apply (simp add: spec_def get_def put_def get_state_def put_state_def high_Env_def)
-  apply (metis Suc_pred le0 le_less_trans less_Suc_eq_le not_less)
-      apply(intro allI; simp)
-     apply (intro get_rule; intro allI; simp)
-      apply (simp add: spec_def get_def put_def get_state_def put_state_def xs_Env_def swap_def)
-     apply(simp add: inc_index_def)
-     apply (intro get_rule; intro allI; simp)
-     apply (simp add: spec_def get_def put_def get_state_def put_state_def i_Env_def)
-    apply(intro allI; simp)
+   apply(intro get_rule; intro allI; clarify)
+  apply(intro seq_rule[of _ _ "(\<lambda>x e. dnfp_precondition e \<and> invariant_low_to_j_is_1_Env e)"])
+    apply(intro cond_rule; simp)
+      apply (smt GG_def One_nat_def case_prodD case_prodI2 inc_lowbound_inv2_aux_def inc_lowbound_inv2_def inc_lowbound_invariantWhite lessI loop_update_action_pre_def spec_def)
+     apply (smt GG_def One_nat_def case_prodD case_prodI2 dec_highbound_inv2_aux_def dec_highbound_inv2_def dec_highbound_invariantWhite loop_update_action_pre_def spec_def)
+  apply (smt GG_def One_nat_def Suc_less_eq inc_index_inv2_aux_def inc_index_inv2_def inc_index_invariantWhite less_Suc_eq loop_update_action_pre_def spec_def split_beta')
   apply blast
     apply(simp add: spec_def)
-  apply(simp add: skip_def)
-  sorry
-
-lemma dnfp_invariantWhite_aux: "spec (\<lambda>e. \<forall>x. low e \<le> x \<and> x < i e \<longrightarrow> xs e ! x = Suc 0) (dnfp_mon v) (\<lambda>x e. \<forall>x. low e \<le> x \<and> x < i e \<longrightarrow> xs e ! x = Suc 0)"
- apply(induction v rule: dnfp_mon.induct)
-    apply(simp add: spec_def)
-    apply (simp add: skip_def)
-  apply(simp only: caseN)
-  apply(intro get_rule; intro allI; clarify)
-  apply(intro cond_rule)
-  apply(simp add: loop_update_action_def)
-  apply(intro get_rule; intro allI; clarify)
-  apply(intro seq_rule[of _ _ "(\<lambda>_ e. i e \<ge> low e \<and> high e \<ge> i e \<and> (\<forall>x. low e \<le> x \<and> x < i e \<longrightarrow> xs e ! x = Suc 0))"])
-  apply(intro cond_rule)
-  apply(simp add: inc_lowbound_def)
-     apply (intro get_rule; intro allI; simp)
-   apply (simp add: spec_def put_def put_state_def  get_state_def xs_Env_def swap_def get_def i_Env_def low_Env_def return_def run_state_def)
-      apply(intro allI)
-      apply (simp add: nth_list_update)
-  defer
-     apply(simp add: dec_highbound_def)
-        apply(intro get_rule; intro allI; simp)
-    apply(intro seq_rule[of _ _ "(\<lambda>x e. low e \<le> i e \<and> high e \<ge> i e \<and> length (xs e) > high e \<and> (\<forall>x. low e \<le> x \<and> x < i e \<longrightarrow> xs e ! x = Suc 0))"])
-       apply (simp add: spec_def put_def put_state_def get_state_def high_Env_def swap_def)
-    apply linarith
-     apply(intro allI; simp)
-    apply(intro get_rule;intro allI; simp)
-       apply (simp add: spec_def put_def put_state_def get_state_def xs_Env_def swap_def)
-  defer
-   apply(simp add: inc_index_def)
-   apply(intro get_rule;intro allI; simp)
-   apply (simp add: spec_def put_def put_state_def get_state_def i_Env_def)
-   apply(intro allI)
-  sorry
-
-lemma dnfp_invariantBlue_aux: "spec (\<lambda>e. \<forall>x \<ge> high e. xs e ! x = 2) (dnfp_mon v) (\<lambda>x e. \<forall>x \<ge> high e. xs e ! x = 2)"
-  sorry
-
-lemma dnfp_invariantRed: "spec (dnfp_inv1 n) (dnfp_mon n) (GG low_invariant_is_0_Env)"
-  unfolding dnfp_inv1_def dnfp_pre_aux_def  GG_def low_invariant_is_0_Env_def
-  apply(induction n rule: dnfp_mon.induct)
-    apply(simp add: spec_def)
-    apply(simp add: skip_def)
-  apply(simp only: caseN)
-   apply(intro get_rule; intro allI; clarify)
-  apply(intro cond_rule)
-  apply(simp add: loop_update_action_def)
-   apply(intro get_rule; intro allI; clarify)
-  apply(intro seq_rule[of _ _ "(\<lambda>x e. \<forall>x<low e. xs e ! x = 0)"])
-  apply(intro cond_rule)
- apply(simp add: inc_lowbound_def)
-     apply (intro get_rule; intro allI; simp)
-  apply(intro seq_rule[of _ _ "(\<lambda>x e. xs e ! low e = 0 \<and>  (\<forall>x<low e. xs e ! x = 0))"])
-      apply (simp add: spec_def put_def put_state_def swap_def get_state_def xs_Env_def)
-   apply auto[1]
-  apply(intro allI; simp)
-  apply(intro get_rule; intro allI)
-  apply(intro seq_rule[of _ _ "(\<lambda>x e. xs e ! low e = 0 \<and> (\<forall>x<low e. xs e ! x = 0))"])
-   apply (simp add: spec_def put_def put_state_def get_state_def i_Env_def)
-  apply(intro allI; simp)
-  apply(intro get_rule; intro allI)
-     apply (simp add: spec_def put_def put_state_def get_state_def low_Env_def)
-   using less_antisym apply blast
-     apply(simp add: dec_highbound_def)
-     apply (intro get_rule; intro allI; simp)
-      apply(intro seq_rule[of _ _ "(\<lambda>x e. (\<forall>x<low e. xs e ! x = 0) \<and> high e \<le> length (xs e) \<and> high e \<ge> i e \<and> low e \<le> i e)"]) 
-       apply (simp add: spec_def get_def put_def get_state_def put_state_def high_Env_def)
-       apply(linarith)
-      apply(intro allI; simp)
-     apply (intro get_rule; intro allI; simp)
-      apply (simp add: spec_def get_def put_def get_state_def put_state_def xs_Env_def swap_def)
-     apply(simp add: inc_index_def)
-     apply (intro get_rule; intro allI; simp)
-     apply (simp add: spec_def get_def put_def get_state_def put_state_def i_Env_def)
-    apply(intro allI; simp)
-   using dnfp_invariantRed_aux apply blast
-    apply(simp add: spec_def)
    by(simp add: skip_def)
 
-lemma dnfp_invariantWhite: "spec (dnfp_inv2 n) (dnfp_mon n) (GG invariant_low_to_j_is_1_Env)"
-  unfolding dnfp_inv2_def dnfp_pre_aux_def  GG_def invariant_low_to_j_is_1_Env_def
+lemma dnfp_invariantBlue: "spec dnfp_inv3 (dnfp_mon n) (GG dnfp_inv3)"
+  unfolding dnfp_inv3_def dnfp_pre_aux_def  GG_def
   apply(induction n rule: dnfp_mon.induct)
     apply(simp add: spec_def)
     apply(simp add: skip_def)
   apply(simp only: caseN)
    apply(intro get_rule; intro allI; clarify)
-  apply(intro cond_rule)
+  apply(intro cond_rule; simp)
   apply(simp add: loop_update_action_def)
    apply(intro get_rule; intro allI; clarify)
-  apply(intro seq_rule[of _ _ "(\<lambda>x e. \<forall>x. low e \<le> x \<and> x < i e \<longrightarrow> xs e ! x = Suc 0)"])
-  apply(intro cond_rule)
-     apply(simp add: inc_lowbound_def)
-     apply (intro get_rule; intro allI; simp)
-   apply (simp add: spec_def put_def put_state_def  get_state_def xs_Env_def swap_def get_def i_Env_def low_Env_def return_def)
-   apply(intro allI)
-     apply (simp add: nth_list_update)
-     apply(simp add: dec_highbound_def)
-        apply(intro get_rule; intro allI; simp)
-    apply(intro seq_rule[of _ _ "(\<lambda>x e. low e \<le> i e \<and> high e \<ge> i e \<and> length (xs e) > high e \<and> (\<forall>x. low e \<le> x \<and> x < i e \<longrightarrow> xs e ! x = Suc 0))"])
-     apply (simp add: spec_def put_def put_state_def get_state_def high_Env_def swap_def)
-    apply linarith
-     apply(intro allI; simp)
-    apply(intro get_rule;intro allI; simp)
-   apply (simp add: spec_def put_def put_state_def get_state_def xs_Env_def swap_def)
-   apply(simp add: inc_index_def)
-   apply(intro get_rule;intro allI; simp)
-   apply (simp add: spec_def put_def put_state_def get_state_def i_Env_def)
-    apply(intro allI)
-    apply (metis Suc_lessI less_SucE)
-    apply(intro allI)
-   using dnfp_invariantWhite_aux apply blast
-    apply(simp add: spec_def)
-   by(simp add: skip_def)
-
-lemma dnfp_invariantBlue: "spec (dnfp_inv3 n) (dnfp_mon n) (GG high_invariant_is_2_Env)"
-  unfolding dnfp_inv3_def dnfp_pre_aux_def  GG_def high_invariant_is_2_Env_def
-  apply(induction n rule: dnfp_mon.induct)
-    apply(simp add: spec_def)
-    apply(simp add: skip_def)
-  apply(simp only: caseN)
-   apply(intro get_rule; intro allI; clarify)
-  apply(intro cond_rule)
-  apply(simp add: loop_update_action_def)
-   apply(intro get_rule; intro allI; clarify)
-  apply(intro seq_rule[of _ _ "(\<lambda>x e. (\<forall>x. high e \<le> x \<and> x < length (xs e) \<longrightarrow> xs e ! x = 2))"])
-   apply (intro cond_rule)
-     apply(simp add: inc_lowbound_def) 
-     apply(intro get_rule;intro allI; simp)
-  apply(intro seq_rule[of _ _ "(\<lambda>x e. \<forall>x. high e \<le> x \<and> x < length (xs e) \<longrightarrow> xs e ! x = 2)"])
-   apply (simp add: spec_def put_def put_state_def swap_def get_state_def xs_Env_def)
-  apply(intro allI; simp)
-  apply(intro get_rule; intro allI)
-  apply(intro seq_rule[of _ _ "(\<lambda>x e. \<forall>x. high e \<le> x \<and> x < length (xs e) \<longrightarrow> xs e ! x = 2)"])
-   apply (simp add: spec_def put_def put_state_def get_state_def i_Env_def)
-  apply(intro allI; simp)
-  apply(intro get_rule; intro allI)
-     apply (simp add: spec_def put_def put_state_def get_state_def low_Env_def)
-    apply(simp_all add: dec_highbound_def)
-     apply(intro get_rule; intro allI)
-     apply (simp add: spec_def put_def put_state_def get_state_def high_Env_def xs_Env_def swap_def get_def)
-     apply(intro allI)
-   defer
-   apply(simp add: inc_index_def)
-    apply(intro get_rule; intro allI; simp)
-     apply (simp add: spec_def put_def put_state_def get_state_def i_Env_def)
-  defer
-  apply(simp add: spec_def)
-   apply(simp add: skip_def)
-   sorry
+  apply(intro seq_rule[of _ _ "(\<lambda>x e. dnfp_precondition e \<and> high_invariant_is_2_Env e)"])
+    apply (intro cond_rule; simp)
+      apply (smt GG_def One_nat_def case_prodD case_prodI2 inc_lowbound_inv3_aux_def inc_lowbound_inv3_def inc_lowbound_invariantBlue lessI loop_update_action_pre_def spec_def)
+     apply (smt GG_def One_nat_def dec_highbound_inv3_aux_def dec_highbound_inv3_def dec_highbound_invariantBlue loop_update_action_pre_def spec_def split_beta')
+  apply (smt GG_def One_nat_def Suc_less_eq inc_index_inv3_aux_def inc_index_inv3_def inc_index_invariantBlue less_Suc_eq loop_update_action_pre_def spec_def split_beta')
+ apply blast
+     apply(simp add: spec_def)
+  by(simp add: skip_def)
 
  text\<open>Main proof\<close>
-definition dnfp_mon_inv :: "nat \<Rightarrow> env \<Rightarrow> bool" where
-"dnfp_mon_inv n e \<equiv> ((dnfp_inv3 n e) \<and>  (dnfp_inv2 n e) \<and> (dnfp_inv1 n e))"
+definition dnfp_mon_inv :: "env \<Rightarrow> bool" where
+"dnfp_mon_inv e \<equiv> ((dnfp_inv3 e) \<and> (dnfp_inv2 e) \<and> (dnfp_inv1 e))"
 
-lemma dnfp_mon_invariants: "spec (dnfp_mon_inv n) (dnfp_mon n) (GG invariants_Env)"
+lemma dnfp_mon_invariants: "spec (dnfp_mon_inv) (dnfp_mon n) (GG dnfp_mon_inv)"
   by (smt GG_def dnfp_invariantBlue dnfp_invariantRed dnfp_invariantWhite dnfp_mon_inv_def invariants_Env_def spec_def split_def)
 
 definition dnfp_post_spec where
-"dnfp_post_spec e \<equiv> invariants_Env e \<and> i e = high e"
+"dnfp_post_spec e \<equiv> dnfp_mon_inv e \<and> i e = high e"
 
 lemma dnfp_mon_isSorted: "dnfp_post_spec e \<Longrightarrow> sorted (xs e)" 
-  unfolding  dnfp_post_spec_def high_invariant_is_2_Env_def invariant_low_to_j_is_1_Env_def invariants_Env_def low_invariant_is_0_Env_def
-  by (smt add_diff_cancel_left' diff_is_0_eq' le_less_trans less_Suc_eq_0_disj  not_less not_less_eq_eq numeral_2_eq_2 plus_1_eq_Suc sorted_iff_nth_mono)
+  unfolding  dnfp_post_spec_def dnfp_mon_inv_def
+  sledgehammer
+  by (smt Suc_1 Suc_leD dnfp_inv1_def dnfp_inv2_def dnfp_inv3_def high_invariant_is_2_Env_def invariant_low_to_j_is_1_Env_def less_numeral_extra(1) less_or_eq_imp_le less_trans low_invariant_is_0_Env_def not_less sorted_iff_nth_mono_less)
 
 definition dnfp_post_spec1 where
-"dnfp_post_spec1 e \<equiv> invariants_Env e \<and> i e = high e \<and> sorted(xs e)"
+"dnfp_post_spec1 e \<equiv> dnfp_mon_inv e \<and> i e = high e \<and> sorted(xs e)"
 
-lemma dnfp_mon_main: "spec (dnfp_mon_inv n) (dnfp_mon n) (GG (dnfp_post_spec1))"
+lemma dnfp_mon_main: "spec (dnfp_mon_inv) (dnfp_mon n) (GG (dnfp_post_spec1))"
   unfolding GG_def dnfp_post_spec1_def
   apply(intro conj_rule_right)
-  apply (metis GG_def dnfp_mon_invariants strengthen_rule)
-  unfolding dnfp_mon_inv_def dnfp_inv3_def dnfp_inv2_def dnfp_inv1_def dnfp_pre_aux_def
-   apply (smt case_prod_beta' dnfp_aux7 spec_def)  
-  by (smt GG_def case_prod_beta' dnfp_aux7 dnfp_inv1_def dnfp_inv2_def dnfp_inv3_def dnfp_mon_inv_def dnfp_mon_invariants dnfp_mon_isSorted dnfp_post_spec_def dnfp_pre_aux_def spec_def)
-
+    apply (metis GG_def dnfp_mon_invariants strengthen_rule)
+   defer
+  sorry
 
 
 end
